parametrize program logic proofs over word impl

bedrock2/src/bedrock2/FE310CSemantics.v
@@ -11,63 +11,72 @@ Local Open Scope string_scope. Local Open Scope Z_scope. Local Open Scope list_s
 Definition MMIOREAD : string := "MMIOREAD".
 Definition MMIOWRITE : string := "MMIOWRITE".
 
-Instance parameters : parameters :=
-  let word := Naive.word32 in
-  let byte := Naive.word8 in
+Module parameters.
+  Class parameters := {
+    word :> Word.Interface.word 32;
+    word_ok :> word.ok word; (* for impl of mem below *)
+    byte :> Word.Interface.word 8;
+    byte_ok :> word.ok byte; (* for impl of mem below *)
+    mem :> Interface.map.map word byte;
+    mem_ok :> Interface.map.ok mem; (* for impl of mem below *)
+  }.
+End parameters. Notation parameters := parameters.parameters.
 
-  {|
-  width := 32;
-  syntax := StringNamesSyntax.make BasicCSyntax.StringNames_params;
-  varname_eqb := String.eqb;
-  funname_eqb := String.eqb;
-  actname_eqb := String.eqb;
-  mem := SortedListWord.map _ _;
-  locals := SortedListString.map _;
-  funname_env := SortedListString.map;
-  ext_spec t m action args post :=
-    if string_dec action MMIOREAD then
-    match args with
-    | [addr] =>
-      ((Ox"10012000" <= word.unsigned addr < Ox"10013000") \/
-       (Ox"10024000" <= word.unsigned addr < Ox"10025000")  )
-      /\ forall v, post m [v]
-    | _ => False
-    end else
-    if string_dec action MMIOWRITE then
-    match args with
-    | [addr; val] =>
-      ((Ox"10012000" <= word.unsigned addr < Ox"10013000") \/
-       (Ox"10024000" <= word.unsigned addr < Ox"10025000")  )
-      /\ post m []
-    |  _ => False
-    end else False;
-|}.
-
-Axiom TODO_andres_differential_memory_log : False.
-Global Instance ok : Semantics.parameters_ok parameters.
-Proof.
-  split; cbv [funname_env locals mem parameters]; try exact _.
-  { cbv; auto. }
-  { eapply SortedListString.ok. }
-  { intros; eapply SortedListString.ok. }
-  split.
-  { case TODO_andres_differential_memory_log. }
-  1,2:
-    cbv [ext_spec parameters]; intros;
-    cbv [Morphisms.Proper Morphisms.respectful Morphisms.pointwise_relation Basics.impl] in *;
-      repeat match goal with |- context [string_dec ?a ?b] => destruct (string_dec a b) end;
-      destruct args as [|? [|? [|]]]; intuition eauto.
-Qed.
-
-(* TODO why does typeclass search fail here? *)
-Instance mapok: Interface.map.ok mem := SortedListWord.ok Naive.word32 _.
-Instance wordok: word.ok Semantics.word := Naive.word32_ok.
-Instance byteok: word.ok Semantics.byte := Naive.word8_ok.
-Add Ring wring : (Properties.word.ring_theory (word := Semantics.word))
-      (preprocess [autorewrite with rew_word_morphism],
-       morphism (Properties.word.ring_morph (word := Semantics.word)),
-       constants [Properties.word_cst]).
-Add Ring bring : (Properties.word.ring_theory (word := Semantics.byte))
-      (preprocess [autorewrite with rew_word_morphism],
-       morphism (Properties.word.ring_morph (word := Semantics.byte)),
-       constants [Properties.word_cst]).
+Section WithParameters.
+  Context {p : parameters}.
+  Global Instance semantics_parameters  : Semantics.parameters :=
+    {|
+    syntax := StringNamesSyntax.make BasicCSyntax.StringNames_params;
+    Semantics.word := parameters.word;
+    Semantics.byte := parameters.byte;
+    varname_eqb := String.eqb;
+    funname_eqb := String.eqb;
+    actname_eqb := String.eqb;
+    mem := parameters.mem;
+    locals := SortedListString.map _;
+    funname_env := SortedListString.map;
+    ext_spec t m action args post :=
+      if string_dec action MMIOREAD then
+      match args with
+      | [addr] =>
+        ((Ox"10012000" <= word.unsigned addr < Ox"10013000") \/
+         (Ox"10024000" <= word.unsigned addr < Ox"10025000")  )
+        /\ forall v, post m [v]
+      | _ => False
+      end else
+      if string_dec action MMIOWRITE then
+      match args with
+      | [addr; val] =>
+        ((Ox"10012000" <= word.unsigned addr < Ox"10013000") \/
+         (Ox"10024000" <= word.unsigned addr < Ox"10025000")  )
+        /\ post m []
+      |  _ => False
+      end else False;
+  |}.
+  
+  Axiom TODO_andres_differential_memory_log : False.
+  Global Instance ok : Semantics.parameters_ok semantics_parameters.
+  Proof.
+    split; cbv [funname_env locals mem semantics_parameters]; try exact _.
+    { cbv; auto. }
+    { exact (SortedListString.ok _). }
+    { exact SortedListString.ok. }
+    split.
+    { case TODO_andres_differential_memory_log. }
+    1,2:
+      cbv [ext_spec semantics_parameters]; intros;
+      cbv [Morphisms.Proper Morphisms.respectful Morphisms.pointwise_relation Basics.impl] in *;
+        repeat match goal with |- context [string_dec ?a ?b] => destruct (string_dec a b) end;
+        destruct args as [|? [|? [|]]]; intuition eauto.
+  Qed.
+  
+  (* COPY-PASTE these *)
+  Add Ring wring : (Properties.word.ring_theory (word := Semantics.word))
+        (preprocess [autorewrite with rew_word_morphism],
+         morphism (Properties.word.ring_morph (word := Semantics.word)),
+         constants [Properties.word_cst]).
+  Add Ring bring : (Properties.word.ring_theory (word := Semantics.byte))
+        (preprocess [autorewrite with rew_word_morphism],
+         morphism (Properties.word.ring_morph (word := Semantics.byte)),
+         constants [Properties.word_cst]).
+End WithParameters.
