bedrock2/src/bedrock2Examples/lightbulb.v
@@ -10,15 +10,11 @@ From coqutil Require Import Word.Interface Map.Interface.
 From coqutil.Tactics Require Import letexists eabstract.
 From bedrock2 Require Import FE310CSemantics Semantics WeakestPrecondition ProgramLogic Array Scalars.
 From bedrock2.Map Require Import Separation SeparationLogic.
-
-Import Syntax BinInt String List.ListNotations ZArith.
-Local Open Scope string_scope. Local Open Scope Z_scope. Local Open Scope list_scope.
-Local Coercion literal (z : Z) : expr := expr.literal z.
-Local Coercion var (x : String.string) : expr := expr.var x.
-Local Coercion name_of_func (f : BasicCSyntax.function) := fst f.
+Import ZArith.
+Local Open Scope Z_scope.
 
 (* TODO: refactor *)
-Lemma word__unsigned_of_Z_nowrap x : 0 <= x < 2 ^ width -> word.unsigned (word.of_Z x) = x.
+Lemma word__unsigned_of_Z_nowrap {width} {word: word.word width} {ok : word.ok word} x : 0 <= x < 2 ^ width -> word.unsigned (word.of_Z x) = x.
 Proof.
   intros. rewrite word.unsigned_of_Z. unfold word.wrap. rewrite Z.mod_small; trivial.
 Qed.
@@ -27,7 +23,7 @@ Local Ltac seplog_use_array_load1 H i :=
   let H0 := fresh in pose proof H as H0;
   unshelve SeparationLogic.seprewrite_in @array_index_nat_inbounds H0;
     [exact iNat|exact (word.of_Z 0)|blia|];
-  change ((word.unsigned (word.of_Z 1) * Z.of_nat iNat)%Z) with i in *.
+  replace ((word.unsigned (word.of_Z 1) * Z.of_nat iNat)%Z) with i in * by (rewrite word.unsigned_of_Z; exact eq_refl).
 Local Ltac trans_ltu :=
   match goal with
   | H : word.unsigned ?v <> 0 |- _ =>
@@ -48,621 +44,660 @@ Local Ltac split_if :=
         end
   end.
 
-Definition lightbulb_loop :=
-    let p_addr : varname := "p_addr" in
-    let bytesWritten : varname := "bytesWritten" in
-    let recvEthernet : varname := "recvEthernet" in
-    let lightbulb_handle : varname := "lightbulb_handle" in
-    let err : varname := "err" in
-
-  ("lightbulb_loop", ((p_addr::nil), (err::nil), bedrock_func_body:(
-    unpack! bytesWritten, err = recvEthernet(p_addr);
-    if !err { (* success, packet *)
-      unpack! err = lightbulb_handle(p_addr, bytesWritten);
-      err = (constr:(0)) (* bad packet continue anyway *)
-    } else if !(err ^ constr:(1)) { (* success, no packet *)
-      err = (constr:(0))
-    }
-  ))).
-
-Definition recvEthernet :=
-    let buf : varname := "buf" in
-    let num_bytes : varname := "num_bytes" in
-    let i : varname := "i" in
-    let err : varname := "err" in
-    let read : varname := "read" in
-
-    ("recvEthernet", ((buf::nil), (num_bytes::err::nil), bedrock_func_body:(
-        num_bytes = (constr:(0));
-        unpack! read, err = lan9250_readword(constr:(Ox"7C")); (* RX_FIFO_INF *)
-        require !err else { err = (constr:(-1)) };
-        require (read & constr:((2^8-1)*2^16)) else { err = (constr:(1)) }; (* nonempty *)
-        unpack! read, err = lan9250_readword(constr:(Ox"40")); (* RX_STATUS_FIFO_PORT *)
-        require !err else { err = (constr:(-1)) };
-
-        num_bytes = (read >> constr:(16) & constr:(2^14-1));
-        (* round up to next word *)
-        num_bytes = ((num_bytes + constr:(4-1)) >> constr:(2));
-        num_bytes = (num_bytes + num_bytes);
-        num_bytes = (num_bytes + num_bytes);
-
-        require (num_bytes < constr:(1520 + 1)) else { err = (constr:(2)) };
-
-        i = (constr:(0)); while (i < num_bytes) {
-            unpack! read, err = lan9250_readword(constr:(0));
-            if err { err = (constr:(-1)); i = (num_bytes) }
-            else { store4(buf + i, read); i = (i + constr:(4)) }
-        }
+Section WithParameters.
+  Context {p : FE310CSemantics.parameters}.
+  Import Syntax BinInt String List.ListNotations ZArith.
+  Local Open Scope string_scope. Local Open Scope Z_scope. Local Open Scope list_scope.
+  Local Coercion literal (z : Z) : expr := expr.literal z.
+  Local Coercion var (x : String.string) : expr := expr.var x.
+  Local Coercion name_of_func (f : BasicCSyntax.function) := fst f.
+  
+  Definition lightbulb_loop :=
+      let p_addr : varname := "p_addr" in
+      let bytesWritten : varname := "bytesWritten" in
+      let recvEthernet : varname := "recvEthernet" in
+      let lightbulb_handle : varname := "lightbulb_handle" in
+      let err : varname := "err" in
+  
+    ("lightbulb_loop", ((p_addr::nil), (err::nil), bedrock_func_body:(
+      unpack! bytesWritten, err = recvEthernet(p_addr);
+      if !err { (* success, packet *)
+        unpack! err = lightbulb_handle(p_addr, bytesWritten);
+        err = (constr:(0)) (* bad packet continue anyway *)
+      } else if !(err ^ constr:(1)) { (* success, no packet *)
+        err = (constr:(0))
+      }
     ))).
-
-Definition lightbulb_handle :=
-    let packet : varname := "packet" in
-    let len : varname := "len" in
-    let ethertype : varname := "ethertype" in
-    let protocol : varname := "protocol" in
-    let port : varname := "port" in
-    let mmio_val : varname := "mmio_val" in
-    let command : varname := "command" in
-    let Oxff : varname := "Oxff" in
-    let MMIOREAD : varname := "MMIOREAD" in
-    let MMIOWRITE : varname := "MMIOWRITE" in
-    let r : varname := "r" in
-
-  ("lightbulb_handle", ((packet::len::nil), (r::nil), bedrock_func_body:(
-    r = (constr:(42));
-    require (r < len) else { r = (constr:(-1)) };
-
-    Oxff = (constr:(Ox"ff"));
-    ethertype = ((((load1(packet + constr:(12)))&Oxff) << constr:(8)) | ((load1(packet + constr:(13)))&Oxff));
-    r = (constr:(1536 - 1));
-    require (r < ethertype) else { r = (constr:(-1)) };
-
-    r = (constr:(23));
-    r = (packet + r);
-    protocol = ((load1(r))&Oxff);
-    r = (constr:(Ox"11"));
-    require (protocol == r) else { r = (constr:(-1)) };
-
-    r = (constr:(42));
-    r = (packet + r);
-    command = ((load1(r))&Oxff);
-    command = (command&constr:(1));
-
-    (* pin output enable -- TODO do this in init
-    io! mmio_val = MMIOREAD(constr:(Ox"10012008"));
-    output! MMIOWRITE(constr:(Ox"10012008"), mmio_val | constr:(2^23));
-    *)
-
-    r = (constr:(Ox"1001200c"));
-    io! mmio_val = MMIOREAD(r);
-    mmio_val = (mmio_val & constr:(Z.clearbit (2^32-1) 23));
-    output! MMIOWRITE(r, mmio_val | command << constr:(23));
-
-    r = (constr:(0))
-  ))).
-
-Definition lightbulb_init :=
-    let err : varname := "err" in
-    let MMIOWRITE : varname := "MMIOWRITE" in
-
-  ("lightbulb_init", (@nil varname, (err::nil), bedrock_func_body:(
-    output! MMIOWRITE(constr:(Ox"10012038"), constr:((Z.shiftl (Ox"f") 2)));
-    output! MMIOWRITE(constr:(Ox"10012008"), constr:((Z.shiftl 1 23)));
-    unpack! err = lan9250_init()
-  ))).
-
-Import Datatypes List.
-Local Notation bytes := (array scalar8 (word.of_Z 1)).
-Local Infix "*" := (sep).
-Local Infix "*" := (sep) : type_scope.
-
-Import TracePredicate. Import TracePredicateNotations.
-Import Word.Properties.
-Import lightbulb_spec.
-
-Instance spec_of_recvEthernet : spec_of "recvEthernet" := fun functions =>
-  forall p_addr (buf:list byte) R m t,
-    (array scalar8 (word.of_Z 1) p_addr buf * R) m ->
-    length buf = 1520%nat ->
-    WeakestPrecondition.call functions "recvEthernet" t m [p_addr] (fun t' m' rets =>
-      exists bytes_written err, rets = [bytes_written; err] /\
-      exists iol, t' = iol ++ t /\
-      exists ioh, mmio_trace_abstraction_relation ioh iol /\ Logic.or
-        (word.unsigned err = 0 /\
-          exists recv buf, (bytes p_addr recv * bytes (word.add p_addr bytes_written) buf * R) m' /\ lan9250_recv _ _ recv ioh /\
-          word.unsigned bytes_written + Z.of_nat (length buf) = 1520%Z /\
-          Z.of_nat (length recv) = word.unsigned bytes_written)
-        (word.unsigned err <> 0 /\ exists buf, (array scalar8 (word.of_Z 1) p_addr buf * R) m' /\ length buf = 1520%nat /\ (
-           word.unsigned err = 1 /\ lan9250_recv_no_packet _ _ ioh \/
-           word.unsigned err = 2 /\ lan9250_recv_packet_too_long _ _ ioh \/
-           word.unsigned err = 2^32-1 /\ TracePredicate.concat TracePredicate.any (spi_timeout word) ioh
-          ))
-      ).
-
-Definition lightbulb_packet_rep cmd (buf : list byte) :=
-  let idx i buf := word.of_Z (word.unsigned (List.hd (word.of_Z 0) (List.skipn i buf))) in
-  42 < Z.of_nat (length buf) /\
-  1535 < word.unsigned ((word.or (word.slu (idx 12%nat buf) (word.of_Z 8)) (idx 13%nat buf))) /\
-  idx 23%nat buf = word.of_Z (Ox"11") /\
-  cmd = Z.testbit (word.unsigned (List.hd (word.of_Z 0) (List.skipn 42 buf))) 0.
-
-Instance spec_of_lightbulb : spec_of "lightbulb_handle" := fun functions =>
-  forall p_addr (buf:list byte) (len:word) R m t,
-    (array scalar8 (word.of_Z 1) p_addr buf * R) m ->
-    word.unsigned len = Z.of_nat (List.length buf) ->
-    WeakestPrecondition.call functions "lightbulb_handle" t m [p_addr; len]
-      (fun t' m' rets => exists v, rets = [v] /\ m' = m /\ 
-      exists iol, t' = iol ++ t /\
-      exists ioh, mmio_trace_abstraction_relation ioh iol /\ Logic.or
-        (exists cmd, lightbulb_packet_rep cmd buf /\ gpio_set _ 23 cmd ioh /\ word.unsigned v = 0)
-        (not (exists cmd, lightbulb_packet_rep cmd buf) /\ ioh = nil /\ word.unsigned v <> 0)
-      ).
-
-Instance spec_of_lightbulb_loop : spec_of "lightbulb_loop" := fun functions =>
-  forall p_addr buf R m t,
-    (bytes p_addr buf * R) m ->
-    Z.of_nat (length buf) = 1520 ->
-    WeakestPrecondition.call functions "lightbulb_loop" t m [p_addr]
-      (fun t' m' rets => exists v, rets = [v] /\
-      (exists buf, (bytes p_addr buf * R) m' /\
-      Z.of_nat (length buf) = 1520) /\
-      exists iol, t' = iol ++ t /\
-      exists ioh, mmio_trace_abstraction_relation ioh iol /\ (
-        (exists packet cmd, (lan9250_recv _ _ packet +++ gpio_set _ 23 cmd) ioh /\ lightbulb_packet_rep cmd packet /\ word.unsigned v = 0) \/
-        (exists packet, (lan9250_recv _ _ packet) ioh /\ not (exists cmd, lightbulb_packet_rep cmd packet) /\ word.unsigned v = 0) \/
-        (lan9250_recv_no_packet _ _ ioh /\ word.unsigned v = 0) \/
-        (lan9250_recv_packet_too_long _ _ ioh /\ word.unsigned v <> 0) \/
-        ((TracePredicate.any +++ (spi_timeout word)) ioh /\ word.unsigned v <> 0)
-      )).
-
-Instance spec_of_lightbulb_init : spec_of "lightbulb_init" := fun functions =>
-  forall m t,
-    WeakestPrecondition.call functions "lightbulb_init" t m nil
-      (fun t' m' rets => exists err, rets = [err] /\ m' = m /\
+  
+  Definition recvEthernet :=
+      let buf : varname := "buf" in
+      let num_bytes : varname := "num_bytes" in
+      let i : varname := "i" in
+      let err : varname := "err" in
+      let read : varname := "read" in
+  
+      ("recvEthernet", ((buf::nil), (num_bytes::err::nil), bedrock_func_body:(
+          num_bytes = (constr:(0));
+          unpack! read, err = lan9250_readword(constr:(Ox"7C")); (* RX_FIFO_INF *)
+          require !err else { err = (constr:(-1)) };
+          require (read & constr:((2^8-1)*2^16)) else { err = (constr:(1)) }; (* nonempty *)
+          unpack! read, err = lan9250_readword(constr:(Ox"40")); (* RX_STATUS_FIFO_PORT *)
+          require !err else { err = (constr:(-1)) };
+  
+          num_bytes = (read >> constr:(16) & constr:(2^14-1));
+          (* round up to next word *)
+          num_bytes = ((num_bytes + constr:(4-1)) >> constr:(2));
+          num_bytes = (num_bytes + num_bytes);
+          num_bytes = (num_bytes + num_bytes);
+  
+          require (num_bytes < constr:(1520 + 1)) else { err = (constr:(2)) };
+  
+          i = (constr:(0)); while (i < num_bytes) {
+              unpack! read, err = lan9250_readword(constr:(0));
+              if err { err = (constr:(-1)); i = (num_bytes) }
+              else { store4(buf + i, read); i = (i + constr:(4)) }
+          }
+      ))).
+  
+  Definition lightbulb_handle :=
+      let packet : varname := "packet" in
+      let len : varname := "len" in
+      let ethertype : varname := "ethertype" in
+      let protocol : varname := "protocol" in
+      let port : varname := "port" in
+      let mmio_val : varname := "mmio_val" in
+      let command : varname := "command" in
+      let Oxff : varname := "Oxff" in
+      let MMIOREAD : varname := "MMIOREAD" in
+      let MMIOWRITE : varname := "MMIOWRITE" in
+      let r : varname := "r" in
+  
+    ("lightbulb_handle", ((packet::len::nil), (r::nil), bedrock_func_body:(
+      r = (constr:(42));
+      require (r < len) else { r = (constr:(-1)) };
+  
+      Oxff = (constr:(Ox"ff"));
+      ethertype = ((((load1(packet + constr:(12)))&Oxff) << constr:(8)) | ((load1(packet + constr:(13)))&Oxff));
+      r = (constr:(1536 - 1));
+      require (r < ethertype) else { r = (constr:(-1)) };
+  
+      r = (constr:(23));
+      r = (packet + r);
+      protocol = ((load1(r))&Oxff);
+      r = (constr:(Ox"11"));
+      require (protocol == r) else { r = (constr:(-1)) };
+  
+      r = (constr:(42));
+      r = (packet + r);
+      command = ((load1(r))&Oxff);
+      command = (command&constr:(1));
+  
+      (* pin output enable -- TODO do this in init
+      io! mmio_val = MMIOREAD(constr:(Ox"10012008"));
+      output! MMIOWRITE(constr:(Ox"10012008"), mmio_val | constr:(2^23));
+      *)
+  
+      r = (constr:(Ox"1001200c"));
+      io! mmio_val = MMIOREAD(r);
+      mmio_val = (mmio_val & constr:(Z.clearbit (2^32-1) 23));
+      output! MMIOWRITE(r, mmio_val | command << constr:(23));
+  
+      r = (constr:(0))
+    ))).
+  
+  Definition lightbulb_init :=
+      let err : varname := "err" in
+      let MMIOWRITE : varname := "MMIOWRITE" in
+  
+    ("lightbulb_init", (@nil varname, (err::nil), bedrock_func_body:(
+      output! MMIOWRITE(constr:(Ox"10012038"), constr:((Z.shiftl (Ox"f") 2)));
+      output! MMIOWRITE(constr:(Ox"10012008"), constr:((Z.shiftl 1 23)));
+      unpack! err = lan9250_init()
+    ))).
+  
+  Import Datatypes List.
+  Local Notation bytes := (array scalar8 (word.of_Z 1)).
+  Local Infix "*" := (sep).
+  Local Infix "*" := (sep) : type_scope.
+  
+  Import TracePredicate. Import TracePredicateNotations.
+  Import Word.Properties.
+  Import lightbulb_spec.
+  
+  Instance spec_of_recvEthernet : spec_of "recvEthernet" := fun functions =>
+    forall p_addr (buf:list byte) R m t,
+      (array scalar8 (word.of_Z 1) p_addr buf * R) m ->
+      length buf = 1520%nat ->
+      WeakestPrecondition.call functions "recvEthernet" t m [p_addr] (fun t' m' rets =>
+        exists bytes_written err, rets = [bytes_written; err] /\
+        exists iol, t' = iol ++ t /\
+        exists ioh, mmio_trace_abstraction_relation ioh iol /\ Logic.or
+          (word.unsigned err = 0 /\
+            exists recv buf, (bytes p_addr recv * bytes (word.add p_addr bytes_written) buf * R) m' /\ lan9250_recv _ _ recv ioh /\
+            word.unsigned bytes_written + Z.of_nat (length buf) = 1520%Z /\
+            Z.of_nat (length recv) = word.unsigned bytes_written)
+          (word.unsigned err <> 0 /\ exists buf, (array scalar8 (word.of_Z 1) p_addr buf * R) m' /\ length buf = 1520%nat /\ (
+             word.unsigned err = 1 /\ lan9250_recv_no_packet _ _ ioh \/
+             word.unsigned err = 2 /\ lan9250_recv_packet_too_long _ _ ioh \/
+             word.unsigned err = 2^32-1 /\ TracePredicate.concat TracePredicate.any (spi_timeout word) ioh
+            ))
+        ).
+  
+  Definition lightbulb_packet_rep cmd (buf : list byte) :=
+    let idx i buf := word.of_Z (word.unsigned (List.hd (word.of_Z 0) (List.skipn i buf))) in
+    42 < Z.of_nat (length buf) /\
+    1535 < word.unsigned ((word.or (word.slu (idx 12%nat buf) (word.of_Z 8)) (idx 13%nat buf))) /\
+    idx 23%nat buf = word.of_Z (Ox"11") /\
+    cmd = Z.testbit (word.unsigned (List.hd (word.of_Z 0) (List.skipn 42 buf))) 0.
+  
+  Instance spec_of_lightbulb : spec_of "lightbulb_handle" := fun functions =>
+    forall p_addr (buf:list byte) (len:word) R m t,
+      (array scalar8 (word.of_Z 1) p_addr buf * R) m ->
+      word.unsigned len = Z.of_nat (List.length buf) ->
+      WeakestPrecondition.call functions "lightbulb_handle" t m [p_addr; len]
+        (fun t' m' rets => exists v, rets = [v] /\ m' = m /\ 
+        exists iol, t' = iol ++ t /\
+        exists ioh, mmio_trace_abstraction_relation ioh iol /\ Logic.or
+          (exists cmd, lightbulb_packet_rep cmd buf /\ gpio_set _ 23 cmd ioh /\ word.unsigned v = 0)
+          (not (exists cmd, lightbulb_packet_rep cmd buf) /\ ioh = nil /\ word.unsigned v <> 0)
+        ).
+  
+  Instance spec_of_lightbulb_loop : spec_of "lightbulb_loop" := fun functions =>
+    forall p_addr buf R m t,
+      (bytes p_addr buf * R) m ->
+      Z.of_nat (length buf) = 1520 ->
+      WeakestPrecondition.call functions "lightbulb_loop" t m [p_addr]
+        (fun t' m' rets => exists v, rets = [v] /\
+        (exists buf, (bytes p_addr buf * R) m' /\
+        Z.of_nat (length buf) = 1520) /\
         exists iol, t' = iol ++ t /\
         exists ioh, mmio_trace_abstraction_relation ioh iol /\ (
-        (lightbulb_boot_success _ _ ioh /\ word.unsigned err = 0) \/
-        (lan9250_boot_timeout  _ _ ioh /\ word.unsigned err <> 0) \/
-        ((TracePredicate.any +++ (spi_timeout word)) ioh /\ word.unsigned err <> 0)
-      )).
-
-
-Require Import bedrock2.AbsintWordToZ.
-Import WeakestPreconditionProperties.
-
-Lemma lightbulb_loop_ok : program_logic_goal_for_function! lightbulb_loop.
-Proof.
-  repeat (match goal with H : or _ _ |- _ => destruct H; intuition idtac end
-        || straightline || straightline_call || split_if || ecancel_assumption || eauto || blia).
-  all : eexists; split; [solve[eauto]|].
-  all : split; [shelve|].
-  all : eexists; split.
-  all: repeat (eapply align_trace_cons || exact (eq_sym (List.app_nil_l _)) || eapply align_trace_app).
-  all : eexists; split.
-  all : repeat (eapply List.Forall2_cons || eapply List.Forall2_refl || eapply List.Forall2_app || eauto 15 using concat_app).
-
-  { subst v. rewrite word.unsigned_xor_nowrap, H10 in H4. case (H4 eq_refl). }
-  { subst v. rewrite word.unsigned_xor_nowrap, H9 in H4. inversion H4. }
-  { subst v. rewrite word.unsigned_xor_nowrap, H9 in H4. inversion H4. }
-
-  Unshelve.
-  all : eexists; split; [ eauto | ].
-  all : try seprewrite_in @bytearray_index_merge H6; eauto.
-  all : try rewrite List.app_length.
-  all : try Lia.lia.
-Qed.
-
-Local Ltac prove_ext_spec :=
-  lazymatch goal with
-  | |- ext_spec _ _ _ _ _ => split; [cbv; clear; firstorder congruence|]; split; [trivial|]
-  end.
-
-Local Ltac zify_unsigned :=
-  repeat match goal with
-  | |- context[word.unsigned ?e] => let H := unsigned.zify_expr e in rewrite H; pose proof H
-  | G : context[word.unsigned ?e] |- _ => let H := unsigned.zify_expr e in rewrite H in G; pose proof H
-  end;
-  repeat match goal with H:absint_eq ?x ?x |- _ => clear H end;
-  repeat match goal with H:?A |- _ => clear H; match goal with G:A |- _ => idtac end end.
-
-Lemma byte_mask_byte (b : Semantics.byte) : word.and (word.of_Z (word.unsigned b)) (word.of_Z 255) = word.of_Z (word.unsigned b) :> Semantics.word.
-Proof.
-  eapply word.unsigned_inj; rewrite word.unsigned_and_nowrap.
-  rewrite !word.unsigned_of_Z.
-  pose proof word.unsigned_range b.
-  cbv [word.wrap].
-  rewrite <-!(Z.land_ones _ width) by (cbv; congruence).
-  rewrite <-word.wrap_unsigned at 2.
-  change (Z.land 255 (Z.ones width)) with (Z.ones 8).
-  change (Z.ones width) with (Z.ones 32).
-  rewrite <-Z.land_ones by blia.
-  Z.bitwise. Btauto.btauto.
-Qed.
-
-Lemma lightbulb_handle_ok : program_logic_goal_for_function! lightbulb_handle.
-Proof.
-  repeat (eauto || straightline || split_if || eapply interact_nomem || prove_ext_spec || trans_ltu).
-  all : subst r; try subst r0; change (word.unsigned (word.of_Z 42)) with 42 in *.
-
-  2: { eexists; split; [solve[eauto]|].
-    split; [solve[eauto]|].
-    eexists nil; split; eauto.
-    eexists nil; split; cbv [mmio_trace_abstraction_relation]; eauto using List.Forall2_refl.
-    right; repeat split; eauto. 
-    { intros (?&?&?). blia. }
-    intros HX; inversion HX. }
-
-  seplog_use_array_load1 H 12.
-  seplog_use_array_load1 H 13.
-  seplog_use_array_load1 H 23.
-  seplog_use_array_load1 H 42.
-  repeat (eauto || straightline || split_if || eapply interact_nomem || prove_ext_spec).
-
-  all : eexists; split; [solve[eauto]|].
-  all : split; [solve[eauto]|].
-  all : eexists; split.
-  all: repeat (eapply align_trace_cons || exact (eq_sym (List.app_nil_l _))).
-  all : eexists; split.
-
-  all : repeat (eapply List.Forall2_cons || eapply List.Forall2_refl).
-  all : 
-  try match goal with
-  |- mmio_event_abstraction_relation _ _ =>
-      (left+right); eexists _, _; split; exact eq_refl
-  end. 
-
-  all : repeat trans_ltu;
-  repeat match goal with
-  | H : word.unsigned ?v <> 0 |- _ =>
-      let v := rdelta.rdelta v in
-      let __ := lazymatch v with if word.eqb _ _ then word.of_Z 1 else word.of_Z 0 => I end in
-      eapply Properties.word.if_nonzero in H; eapply word.eqb_true in H
-  | H : word.unsigned ?v = 0 |- _ =>
-      let v := rdelta.rdelta v in
-      let __ := lazymatch v with if word.eqb _ _ then word.of_Z 1 else word.of_Z 0 => I end in
-      eapply Word.Properties.word.if_zero in H; eapply word.eqb_false in H
-  end;
-  repeat match goal with x := _ |- _ => subst x end;
-  repeat match goal with H : _ |- _ => rewrite !byte_mask_byte in H end.
-  all : repeat straightline.
-
-  1: {
-    left.
-    eexists; repeat split.
-    all : try eassumption.
-    1: blia.
-    cbv [gpio_set one existsl concat].
-    eexists _, ([_]), ([_]); repeat split; repeat f_equal.
-    eapply word.unsigned_inj.
-    rewrite ?byte_mask_byte.
-    rewrite ?word.unsigned_and_nowrap.
-    change (word.unsigned (word.of_Z 1)) with (Z.ones 1).
-    rewrite Z.land_ones, Z.bit0_mod by blia.
-    rewrite !word.unsigned_of_Z.
-    cbv [word.wrap]; change width with 32 in *.
-    rewrite 2(Z.mod_small _ (2^32)); try exact eq_refl.
-    1: match goal with |- 0 <= word.unsigned ?x < _ => pose proof word.unsigned_range x end; blia.
-    clear; Z.div_mod_to_equations; blia. }
-
-  (* parse failures *)
-  all : right; repeat split; eauto; try solve[intros HX; inversion HX]; intros (?&?&?&?&?).
-  all : cbn in *; congruence.
-
-  Unshelve.
-  all : intros; exact True.
-Qed.
-
-
-Lemma recvEthernet_ok : program_logic_goal_for_function! recvEthernet.
-Proof.
-  straightline.
-  rename H into Hcall; clear H0 H1. rename H2 into H. rename H3 into H0.
-  repeat (straightline || split_if || straightline_call || eauto 99 || prove_ext_spec).
-  1, 3: cbv - [Z.le Z.lt]; clear; blia.
-
-  3: {
-
-  refine (TailRecursion.tailrec_earlyout
-    (HList.polymorphic_list.cons (list byte) (HList.polymorphic_list.cons (mem -> Prop) HList.polymorphic_list.nil))
-    ["buf";"num_bytes";"i";"read";"err"]
-    (fun v scratch R t m buf num_bytes_loop i read err => PrimitivePair.pair.mk (
-      word.unsigned err = 0 /\
-      word.unsigned i <= word.unsigned num_bytes /\
-      v = word.unsigned i /\
-      (bytes (word.add buf i) scratch * R) m /\
-      Z.of_nat (List.length scratch) = word.unsigned (word.sub num_bytes i) /\
-      word.unsigned i mod 4 = word.unsigned num_bytes mod 4 /\
-      num_bytes_loop = num_bytes)
-    (fun T M BUF NUM_BYTES I READ ERR =>
-       NUM_BYTES = num_bytes_loop /\
-       exists RECV,
-       (bytes (word.add buf i) RECV * R) M /\
-       List.length RECV = List.length scratch /\
-       exists iol, T = iol ++ t /\
-       exists ioh, mmio_trace_abstraction_relation ioh iol /\
-       (word.unsigned ERR = 0 /\ lan9250_readpacket _ _ RECV ioh \/
-        word.unsigned ERR = 2^32-1 /\ TracePredicate.concat TracePredicate.any (spi_timeout word) ioh ) )
-    )
-    _ _ _ _ _ _ _ _);
-  (* TODO wrap this into a tactic with the previous refine? *)
-  cbn [HList.hlist.foralls HList.tuple.foralls
-       HList.hlist.existss HList.tuple.existss
-       HList.hlist.apply  HList.tuple.apply
-       HList.hlist
-       List.repeat Datatypes.length
-       HList.polymorphic_list.repeat HList.polymorphic_list.length
-       PrimitivePair.pair._1 PrimitivePair.pair._2] in *;
-    repeat (straightline || split_if || eapply interact_nomem || eauto 99).
-  { exact (Z.gt_wf (word.unsigned num_bytes)). }
-  1: repeat (refine (conj _ _)); eauto.
-  { eapply Properties.word.unsigned_range. }
-  1: zify_unsigned.
-  1: replace (word.add p_addr i) with p_addr by (subst i; ring).
-  1: rewrite <- (List.firstn_skipn (Z.to_nat (word.unsigned (word.sub num_bytes i) ) )  _) in H.
-  1: SeparationLogic.seprewrite_in (symmetry! @bytearray_index_merge) H; [|ecancel_assumption].
-    1,2,3:
-    repeat match goal with
-    | |- ?x = ?x => exact (eq_refl x)
-    | _ => progress trans_ltu
-    | _ => progress zify_unsigned
-    | _ => progress rewrite ?Znat.Z2Nat.id by blia
-    | H: _ |- _ => progress (rewrite ?Znat.Z2Nat.id in H by blia)
-    | _ => rewrite List.length_firstn_inbounds by (PreOmega.zify; rewrite ?Znat.Z2Nat.id by blia; blia)
-    | _ => progress rewrite ?Z.sub_0_r
-    end; repeat straightline.
-    { repeat match goal with x:= _ |- context[?x]  => subst x end. clear. Z.div_mod_to_equations. blia. }
-
-    { straightline_call; repeat straightline.
-      { cbv; clear; intuition congruence. }
-      split_if; do 6 straightline.
-
-      (* SPI timeout, break loop *)
-      { straightline.
-        straightline.
-        straightline.
-        straightline.
-        (* [repeat straightline] hangs *)
-        do 5 eexists; split; [repeat straightline|]; [].
-        left.
-        repeat straightline.
-        { subst br0. rewrite word.unsigned_ltu, Z.ltb_irrefl; exact eq_refl. }
-        split; eauto.
-        eexists; split; eauto.
-        split; eauto.
-        eexists; split.
-        { subst a; eauto. }
-        eexists; split; eauto.
-        right; split.
-        { exact eq_refl. }
-        intuition eauto. }
-        
-      (* store *)
-      do 4 straightline.
-      trans_ltu.
-      match goal with
-        | H: context[word.unsigned (word.sub ?a ?b)] |- _ =>
-            pose proof Properties.word.unsigned_range a;
-            pose proof Properties.word.unsigned_range b;
-            let H := fresh in
-            pose proof word.unsigned_sub a b as H;
-            unfold word.wrap in H;
-            rewrite Z.mod_small in H by blia
-      end.
-      match goal with H10 : _ ?a0 |- store _ ?a0 _ _ _ => rewrite <- (List.firstn_skipn 4 _) in H10;
-        SeparationLogic.seprewrite_in (symmetry! @bytearray_index_merge) H10 end.
-      { instantiate (1:= word.of_Z 4). rewrite List.length_firstn_inbounds; [exact eq_refl|]. Z.div_mod_to_equations. blia. }
-      eapply store_four_of_sep.
-      { match goal with H8:_|-_ => seprewrite_in @scalar32_of_bytes H8; [..|ecancel_assumption]; try exact _; [] end.
-        eapply List.length_firstn_inbounds; Z.div_mod_to_equations; blia. }
-
-      (* after store *)
-      do 5 straightline.
-      (* TODO straightline hangs in TailRecursion.enforce *)
-      do 5 letexists. split. { repeat straightline. }
-      right. do 3 letexists.
-      repeat split; repeat straightline; repeat split.
-      { intuition idtac. }
-      { subst i.
-        rewrite word.unsigned_add; cbv [word.wrap]; rewrite Z.mod_small;
-        change (word.unsigned (word.of_Z 4)) with 4; try (Z.div_mod_to_equations; blia). }
-      { replace (word.add x9 i)
-          with (word.add (word.add x9 x11) (word.of_Z 4)) by (subst i; ring).
-        ecancel_assumption. }
-      { repeat match goal with x1 := _ |- _ => subst x1; rewrite List.length_skipn; rewrite Znat.Nat2Z.inj_sub end.
-        { repeat match goal with H5:_|-_=>rewrite H5 end; subst i.
-          progress replace (word.sub num_bytes (word.add x11 (word.of_Z 4)))
-            with (word.sub (word.sub num_bytes x11) (word.of_Z 4)) by ring.
-          rewrite (word.unsigned_sub _ (word.of_Z 4)).
-          unfold word.wrap. rewrite Z.mod_small.
-          all: change (word.unsigned (word.of_Z 4)) with 4; change (Z.of_nat 4) with 4.
-          all : Z.div_mod_to_equations; blia. }
-        Z.div_mod_to_equations; blia. }
-      { subst i.
-        rewrite word.unsigned_add. unfold word.wrap. rewrite (Z.mod_small _ (2 ^ width)).
-        { revert dependent x11. clear. change (word.unsigned (word.of_Z 4)) with 4. intros.
-          Z.div_mod_to_equations. blia. }
-        change (word.unsigned (word.of_Z 4)) with 4.
-        Z.div_mod_to_equations.
-        blia. }
-      { repeat match goal with |- context [?x] => is_var x; subst x end.
-        rewrite word.unsigned_add. unfold word.wrap. rewrite Z.mod_small.
-        { change (word.unsigned (word.of_Z 4)) with 4. blia. }
-        change (word.unsigned (word.of_Z 4)) with 4. Z.div_mod_to_equations. blia. }
-      { subst v'. subst i.
-        rewrite word.unsigned_add. change (word.unsigned (word.of_Z 4)) with 4.
-        unfold word.wrap. rewrite (Z.mod_small _ (2 ^ width));
-          change (2^width) with (2^32) in *; Z.div_mod_to_equations; blia. }
-
-      { letexists; repeat split.
-        { repeat match goal with x := _ |- _ => is_var x; subst x end; subst.
-          cbv [scalar32 truncated_scalar littleendian ptsto_bytes.ptsto_bytes] in *.
-          progress replace (word.add x9 (word.add x11 (word.of_Z 4))) with
-                  (word.add (word.add x9 x11) (word.of_Z 4)) in * by ring.
-          SeparationLogic.seprewrite_in (@bytearray_index_merge) H25.
-          { exact eq_refl. } { ecancel_assumption. } }
-        { subst RECV. rewrite List.app_length.
-          rewrite H26. subst x22. rewrite List.length_skipn.
-          unshelve erewrite (_ : length (HList.tuple.to_list _) = 4%nat); [exact eq_refl|].
-          enough ((4 <= length x7)%nat) by blia.
-          Z.div_mod_to_equations; blia. }
-        repeat match goal with x := _ |- _ => is_var x; subst x end; subst.
-        eexists; split.
-        { rewrite List.app_assoc; eauto. }
-        eexists; split.
-        { eapply List.Forall2_app; eauto.  }
-        destruct H29; [left|right]; repeat (straightline || split || eauto using TracePredicate__any_app_more).
-        eapply TracePredicate.concat_app; eauto.
-        unshelve erewrite (_ : LittleEndian.combine _ _ = word.unsigned x10); rewrite !word.of_Z_unsigned; try solve [intuition idtac].
-        1: replace (word.unsigned x10) with (word.unsigned x10 mod 2^(Z.of_nat (bytes_per (width:=32) access_size.four)*8)).
-        1:rewrite <-LittleEndian.combine_split; f_equal.
-        eapply Properties.word.wrap_unsigned. } }
-
-    { split; eauto. eexists; split; eauto. split; eauto. exists nil; split; eauto.
-      eexists; split; [constructor|].
-      left. split; eauto.
-      enough (Hlen : length x7 = 0%nat) by (destruct x7; try solve[inversion Hlen]; exact eq_refl).
-      PreOmega.zify.
-      rewrite H13.
-      subst br.
-      rewrite word.unsigned_ltu in H11.
-      destruct (word.unsigned x11 <? word.unsigned num_bytes) eqn:HJ; try solve [inversion H11].
-      eapply Z.ltb_nlt in HJ.
-      revert dependent x7; revert dependent num_bytes; revert dependent x11; clear; intros.
-      unshelve erewrite (_:x11 = num_bytes) in *.
-      { eapply Properties.word.unsigned_inj. Z.div_mod_to_equations; Lia.lia. }
-      rewrite word.unsigned_sub, Z.sub_diag; exact eq_refl. }
-    repeat straightline.
-    repeat letexists. split. { repeat straightline. }
-    eexists _, _. split. { exact eq_refl. }
-
-    repeat straightline.
-    subst i.
-    match goal with H: _ |- _ =>
-      progress repeat (unshelve erewrite (_ : forall x, word.add x (word.of_Z 0) = x) in H; [intros; ring|]);
-      progress repeat (unshelve erewrite (_ : forall x, word.sub x (word.of_Z 0) = x) in H; [intros; ring|])
+          (exists packet cmd, (lan9250_recv _ _ packet +++ gpio_set _ 23 cmd) ioh /\ lightbulb_packet_rep cmd packet /\ word.unsigned v = 0) \/
+          (exists packet, (lan9250_recv _ _ packet) ioh /\ not (exists cmd, lightbulb_packet_rep cmd packet) /\ word.unsigned v = 0) \/
+          (lan9250_recv_no_packet _ _ ioh /\ word.unsigned v = 0) \/
+          (lan9250_recv_packet_too_long _ _ ioh /\ word.unsigned v <> 0) \/
+          ((TracePredicate.any +++ (spi_timeout word)) ioh /\ word.unsigned v <> 0)
+        )).
+  
+  Instance spec_of_lightbulb_init : spec_of "lightbulb_init" := fun functions =>
+    forall m t,
+      WeakestPrecondition.call functions "lightbulb_init" t m nil
+        (fun t' m' rets => exists err, rets = [err] /\ m' = m /\
+          exists iol, t' = iol ++ t /\
+          exists ioh, mmio_trace_abstraction_relation ioh iol /\ (
+          (lightbulb_boot_success _ _ ioh /\ word.unsigned err = 0) \/
+          (lan9250_boot_timeout  _ _ ioh /\ word.unsigned err <> 0) \/
+          ((TracePredicate.any +++ (spi_timeout word)) ioh /\ word.unsigned err <> 0)
+        )).
+  
+  
+  Require Import bedrock2.AbsintWordToZ.
+  Import WeakestPreconditionProperties.
+  
+  Lemma lightbulb_loop_ok : program_logic_goal_for_function! lightbulb_loop.
+  Proof.
+    repeat (match goal with H : or _ _ |- _ => destruct H; intuition idtac end
+          || straightline || straightline_call || split_if || ecancel_assumption || eauto || blia).
+    all : eexists; split; [solve[eauto]|].
+    all : split; [shelve|].
+    all : eexists; split.
+    all: repeat (eapply align_trace_cons || exact (eq_sym (List.app_nil_l _)) || eapply align_trace_app).
+    all : eexists; split.
+    all : try subst err; rewrite ?word.unsigned_of_Z.
+    all : repeat (eapply List.Forall2_cons || eapply List.Forall2_refl || eapply List.Forall2_app || eauto 15 using concat_app).
+    { subst v. rewrite word.unsigned_xor_nowrap, H10, word.unsigned_of_Z in H4. case (H4 eq_refl). }
+    { subst v. rewrite word.unsigned_xor_nowrap, H9, word.unsigned_of_Z in H4. inversion H4. }
+    { subst v. rewrite word.unsigned_xor_nowrap, H9, word.unsigned_of_Z in H4. inversion H4. }
+  
+    Unshelve.
+    all : eexists; split; [ eauto | ].
+    all : try seprewrite_in @bytearray_index_merge H6; eauto.
+    all : try rewrite List.app_length.
+    all : try Lia.lia.
+  Qed.
+  
+  Local Ltac prove_ext_spec :=
+    lazymatch goal with
+    | |- ext_spec _ _ _ _ _ => split; [shelve|]; split; [trivial|]
     end.
-    eexists; split.
-    1: { repeat match goal with |- context [?x] => match type of x with list _ => subst x end end.
-      repeat rewrite List.app_assoc. f_equal. }
-    eexists; split.
-    1:repeat eapply List.Forall2_app; eauto.
-    destruct H14; [left|right]; repeat straightline; repeat split; eauto.
-    { trans_ltu; change (word.unsigned (word.of_Z 1521)) with 1521 in *; eexists _, _; repeat split.
-      { SeparationLogic.ecancel_assumption. }
-      { revert dependent x2. revert dependent x6. intros.
-        destruct H5; repeat straightline; try contradiction.
-        destruct H9; repeat straightline; try contradiction.
-        eexists _, _; split.
-        { rewrite <-!List.app_assoc. eauto using concat_app. }
-        split; [zify_unsigned; eauto|].
-      { cbv beta delta [lan9250_decode_length].
-        rewrite H11. rewrite List.firstn_length, Znat.Nat2Z.inj_min.
-        replace (word.sub num_bytes (word.of_Z 0)) with num_bytes by ring.
-        rewrite ?Znat.Z2Nat.id by eapply word.unsigned_range.
-        transitivity (word.unsigned num_bytes); [blia|exact eq_refl]. } }
-      { pose proof word.unsigned_range num_bytes.
-        rewrite length_skipn.
-        PreOmega.zify. rewrite ?Znat.Z2Nat.id in * by blia; blia. }
-      rewrite H11, length_firstn_inbounds, ?Znat.Z2Nat.id.
-      all : try (zify_unsigned;
-      try Lia.lia;
-      eapply Znat.Nat2Z.inj_le;
-      rewrite ?Znat.Z2Nat.id; Lia.lia).
-      }
-    { repeat match goal with H : _ |- _ => rewrite H; intro HX; solve[inversion HX] end. }
-    { trans_ltu; change (word.unsigned (word.of_Z 1521)) with 1521 in *.
-      eexists _; split; eauto; repeat split; try Lia.lia.
-      { SeparationLogic.seprewrite_in @bytearray_index_merge H10.
-        { rewrite H11.
-          1: replace (word.sub num_bytes (word.of_Z 0)) with num_bytes by ring.
-          rewrite List.length_firstn_inbounds, ?Znat.Z2Nat.id.
-          1:exact eq_refl.
-          1:eapply word.unsigned_range.
-          PreOmega.zify.
-          rewrite ?Znat.Z2Nat.id by eapply word.unsigned_range.
+  
+  Local Ltac zify_unsigned :=
+    repeat match goal with
+    | |- context[word.unsigned ?e] => let H := unsigned.zify_expr e in rewrite H; pose proof H
+    | G : context[word.unsigned ?e] |- _ => let H := unsigned.zify_expr e in rewrite H in G; pose proof H
+    end;
+    repeat match goal with H:absint_eq ?x ?x |- _ => clear H end;
+    repeat match goal with H:?A |- _ => clear H; match goal with G:A |- _ => idtac end end.
+  
+  Lemma byte_mask_byte (b : Semantics.byte) : word.and (word.of_Z (word.unsigned b)) (word.of_Z 255) = word.of_Z (word.unsigned b) :> Semantics.word.
+  Proof.
+    eapply word.unsigned_inj; rewrite word.unsigned_and_nowrap.
+    rewrite !word.unsigned_of_Z.
+    pose proof word.unsigned_range b.
+    cbv [word.wrap].
+    rewrite <-!(Z.land_ones _ width) by (cbv; congruence).
+    rewrite <-word.wrap_unsigned at 2.
+    change (Z.land 255 (Z.ones width)) with (Z.ones 8).
+    change (Z.ones width) with (Z.ones 32).
+    rewrite <-Z.land_ones by blia.
+    Z.bitwise. Btauto.btauto.
+  Qed.
+  
+  Lemma lightbulb_handle_ok : program_logic_goal_for_function! lightbulb_handle.
+  Proof.
+    repeat (eauto || straightline || split_if || eapply interact_nomem || prove_ext_spec || trans_ltu).
+    all : subst r; try subst r0; replace (word.unsigned (word.of_Z 42)) with 42 in *.
+    2,4: rewrite word.unsigned_of_Z; exact eq_refl.
+  
+    2: { eexists; split; [solve[eauto]|].
+      split; [solve[eauto]|].
+      eexists nil; split; eauto.
+      eexists nil; split; cbv [mmio_trace_abstraction_relation]; eauto using List.Forall2_refl.
+      right; repeat split; eauto. 
+      { intros (?&?&?). blia. }
+      intros HX; rewrite ?word.unsigned_of_Z in HX; inversion HX. }
+  
+    seplog_use_array_load1 H 12.
+    seplog_use_array_load1 H 13.
+    seplog_use_array_load1 H 23.
+    seplog_use_array_load1 H 42.
+    unshelve (repeat (eauto || straightline || split_if || eapply interact_nomem || prove_ext_spec)).
+    1,2:shelve.
+    1,2: case TODO_andres_mmioaddr.
+  
+    all : eexists; split; [solve[eauto]|].
+    all : split; [solve[eauto]|].
+    all : eexists; split.
+    all: repeat (eapply align_trace_cons || exact (eq_sym (List.app_nil_l _))).
+    all : eexists; split.
+  
+    all : repeat (eapply List.Forall2_cons || eapply List.Forall2_refl).
+    all : 
+    try match goal with
+    |- mmio_event_abstraction_relation _ _ =>
+        (left+right); eexists _, _; split; exact eq_refl
+    end. 
+  
+    all : repeat trans_ltu;
+    repeat match goal with
+    | H : word.unsigned ?v <> 0 |- _ =>
+        let v := rdelta.rdelta v in
+        let __ := lazymatch v with if word.eqb _ _ then word.of_Z 1 else word.of_Z 0 => I end in
+        eapply Properties.word.if_nonzero in H; eapply word.eqb_true in H
+    | H : word.unsigned ?v = 0 |- _ =>
+        let v := rdelta.rdelta v in
+        let __ := lazymatch v with if word.eqb _ _ then word.of_Z 1 else word.of_Z 0 => I end in
+        eapply Word.Properties.word.if_zero in H; eapply word.eqb_false in H
+    end;
+    repeat match goal with x := _ |- _ => subst x end;
+    repeat match goal with H : _ |- _ => rewrite !byte_mask_byte in H end.
+    all : repeat straightline.
+  
+    1: {
+      left.
+      eexists; repeat split.
+      all : rewrite ?word.unsigned_of_Z in H2.
+      all : try eassumption.
+      1: blia.
+      2: eapply word.unsigned_of_Z.
+      cbv [gpio_set one existsl concat].
+      eexists _, ([_]), ([_]); repeat split; repeat f_equal.
+      eapply word.unsigned_inj.
+      rewrite ?byte_mask_byte.
+      rewrite ?word.unsigned_and_nowrap.
+      replace (word.unsigned (word.of_Z 1)) with (Z.ones 1) by (rewrite word.unsigned_of_Z; exact eq_refl).
+      rewrite Z.land_ones, Z.bit0_mod by blia.
+      rewrite !word.unsigned_of_Z.
+      cbv [word.wrap]; change width with 32 in *.
+      rewrite 2(Z.mod_small _ (2^32)); try exact eq_refl.
+      1: match goal with |- 0 <= word.unsigned ?x < _ => pose proof word.unsigned_range x end; blia.
+      clear; Z.div_mod_to_equations; blia. }
+  
+    (* parse failures *)
+    all : right; repeat split; eauto.
+    2,4: rewrite word.unsigned_of_Z; intro X; inversion X.
+    all : intros (?&?&?&?&?).
+    { rewrite H10 in H3. apply H3. exact eq_refl. }
+    { rewrite word.unsigned_of_Z in H2; contradiction. }
+  
+    Unshelve.
+    all : intros; exact True.
+  Qed.
+
+  Add Ring wring : (Properties.word.ring_theory (word := Semantics.word))
+        (preprocess [autorewrite with rew_word_morphism],
+         morphism (Properties.word.ring_morph (word := Semantics.word)),
+         constants [Properties.word_cst]).
+  Add Ring bring : (Properties.word.ring_theory (word := Semantics.byte))
+        (preprocess [autorewrite with rew_word_morphism],
+         morphism (Properties.word.ring_morph (word := Semantics.byte)),
+         constants [Properties.word_cst]).
+  
+  Lemma recvEthernet_ok : program_logic_goal_for_function! recvEthernet.
+  Proof.
+    straightline.
+    rename H into Hcall; clear H0 H1. rename H2 into H. rename H3 into H0.
+    repeat (straightline || split_if || straightline_call || eauto 99 || prove_ext_spec).
+    1, 3: rewrite word.unsigned_of_Z; cbv - [Z.le Z.lt]; clear; blia.
+  
+    3: {
+  
+    refine (TailRecursion.tailrec_earlyout
+      (HList.polymorphic_list.cons (list byte) (HList.polymorphic_list.cons (mem -> Prop) HList.polymorphic_list.nil))
+      ["buf";"num_bytes";"i";"read";"err"]
+      (fun v scratch R t m buf num_bytes_loop i read err => PrimitivePair.pair.mk (
+        word.unsigned err = 0 /\
+        word.unsigned i <= word.unsigned num_bytes /\
+        v = word.unsigned i /\
+        (bytes (word.add buf i) scratch * R) m /\
+        Z.of_nat (List.length scratch) = word.unsigned (word.sub num_bytes i) /\
+        word.unsigned i mod 4 = word.unsigned num_bytes mod 4 /\
+        num_bytes_loop = num_bytes)
+      (fun T M BUF NUM_BYTES I READ ERR =>
+         NUM_BYTES = num_bytes_loop /\
+         exists RECV,
+         (bytes (word.add buf i) RECV * R) M /\
+         List.length RECV = List.length scratch /\
+         exists iol, T = iol ++ t /\
+         exists ioh, mmio_trace_abstraction_relation ioh iol /\
+         (word.unsigned ERR = 0 /\ lan9250_readpacket _ _ RECV ioh \/
+          word.unsigned ERR = 2^32-1 /\ TracePredicate.concat TracePredicate.any (spi_timeout word) ioh ) )
+      )
+      _ _ _ _ _ _ _ _);
+    (* TODO wrap this into a tactic with the previous refine? *)
+    cbn [HList.hlist.foralls HList.tuple.foralls
+         HList.hlist.existss HList.tuple.existss
+         HList.hlist.apply  HList.tuple.apply
+         HList.hlist
+         List.repeat Datatypes.length
+         HList.polymorphic_list.repeat HList.polymorphic_list.length
+         PrimitivePair.pair._1 PrimitivePair.pair._2] in *;
+      repeat (straightline || split_if || eapply interact_nomem || eauto 99).
+    { exact (Z.gt_wf (word.unsigned num_bytes)). }
+    1: repeat (refine (conj _ _)); eauto.
+    { subst i. rewrite word.unsigned_of_Z.
+      eapply Properties.word.unsigned_range. }
+    1: zify_unsigned.
+    1: replace (word.add p_addr i) with p_addr by (subst i; ring).
+    1: rewrite <- (List.firstn_skipn (Z.to_nat (word.unsigned (word.sub num_bytes i) ) )  _) in H.
+    1: SeparationLogic.seprewrite_in (symmetry! @bytearray_index_merge) H; [|ecancel_assumption].
+      1,2,3:
+      repeat match goal with
+      | |- ?x = ?x => exact (eq_refl x)
+      | _ => progress trans_ltu
+      | _ => progress zify_unsigned
+      | _ => progress rewrite ?Znat.Z2Nat.id by blia
+      | H: _ |- _ => progress (rewrite ?Znat.Z2Nat.id in H by blia)
+      | _ => rewrite List.length_firstn_inbounds by (PreOmega.zify; rewrite ?Znat.Z2Nat.id by blia; blia)
+      | _ => progress rewrite ?Z.sub_0_r
+      end; repeat straightline.
+      { repeat match goal with x:= _ |- context[?x]  => subst x end. clear. Z.div_mod_to_equations. blia. }
+  
+      { straightline_call; repeat straightline.
+        { rewrite word.unsigned_of_Z. cbv; clear. intuition congruence. }
+        split_if; do 6 straightline.
+  
+        (* SPI timeout, break loop *)
+        { straightline.
+          straightline.
+          straightline.
+          straightline.
+          (* [repeat straightline] hangs *)
+          do 5 eexists; split; [repeat straightline|]; [].
+          left.
+          repeat straightline.
+          { subst br0. rewrite word.unsigned_ltu, Z.ltb_irrefl, word.unsigned_of_Z; exact eq_refl. }
+          split; eauto.
+          eexists; split; eauto.
+          split; eauto.
+          eexists; split.
+          { subst a; eauto. }
+          eexists; split; eauto.
+          right; split.
+          { subst err. rewrite word.unsigned_of_Z. exact eq_refl. }
+          intuition eauto. }
+          
+        (* store *)
+        do 4 straightline.
+        trans_ltu.
+        match goal with
+          | H: context[word.unsigned (word.sub ?a ?b)] |- _ =>
+              pose proof Properties.word.unsigned_range a;
+              pose proof Properties.word.unsigned_range b;
+              let H := fresh in
+              pose proof word.unsigned_sub a b as H;
+              unfold word.wrap in H;
+              rewrite Z.mod_small in H by blia
+        end.
+        match goal with H10 : _ ?a0 |- store _ ?a0 _ _ _ => rewrite <- (List.firstn_skipn 4 _) in H10;
+          SeparationLogic.seprewrite_in (symmetry! @bytearray_index_merge) H10 end.
+        { instantiate (1:= word.of_Z 4).
+          rewrite word.unsigned_of_Z.
+          rewrite List.length_firstn_inbounds; [exact eq_refl|]. Z.div_mod_to_equations. blia. }
+        eapply store_four_of_sep.
+        { match goal with H8:_|-_ => seprewrite_in @scalar32_of_bytes H8; [..|ecancel_assumption]; try exact _; [] end.
+          eapply List.length_firstn_inbounds; Z.div_mod_to_equations; blia. }
+  
+        (* after store *)
+        do 5 straightline.
+        (* TODO straightline hangs in TailRecursion.enforce *)
+        do 5 letexists. split. { repeat straightline. }
+        right. do 3 letexists.
+        repeat split; repeat straightline; repeat split.
+        { intuition idtac. }
+        { subst i.
+          rewrite word.unsigned_add; cbv [word.wrap]; rewrite Z.mod_small;
+          replace (word.unsigned (word.of_Z 4)) with 4.
+          2,4: rewrite word.unsigned_of_Z; exact eq_refl.
+          1,2: try (Z.div_mod_to_equations; blia). }
+        { replace (word.add x9 i)
+            with (word.add (word.add x9 x11) (word.of_Z 4)) by (subst i; ring).
+          ecancel_assumption. }
+        { repeat match goal with x1 := _ |- _ => subst x1; rewrite List.length_skipn; rewrite Znat.Nat2Z.inj_sub end.
+          { repeat match goal with H5:_|-_=>rewrite H5 end; subst i.
+            progress replace (word.sub num_bytes (word.add x11 (word.of_Z 4)))
+              with (word.sub (word.sub num_bytes x11) (word.of_Z 4)) by ring.
+            rewrite (word.unsigned_sub _ (word.of_Z 4)).
+            unfold word.wrap. rewrite Z.mod_small.
+            all: replace (word.unsigned (word.of_Z 4)) with 4 by (rewrite word.unsigned_of_Z; exact eq_refl).
+            all: change (Z.of_nat 4) with 4.
+            all : Z.div_mod_to_equations; blia. }
+          Z.div_mod_to_equations; blia. }
+        { subst i.
+          rewrite word.unsigned_add. unfold word.wrap. rewrite (Z.mod_small _ (2 ^ width)).
+          { revert dependent x11. clear.
+            replace (word.unsigned (word.of_Z 4)) with 4 by (rewrite word.unsigned_of_Z; exact eq_refl).
+            intros.
+            Z.div_mod_to_equations. blia. }
+          replace (word.unsigned (word.of_Z 4)) with 4 by (rewrite word.unsigned_of_Z; exact eq_refl).
+          Z.div_mod_to_equations.
           blia. }
-        eapply H15. }
-      { 1:rewrite List.app_length, List.length_skipn, H11, List.firstn_length.
-        replace (word.sub num_bytes (word.of_Z 0)) with num_bytes by ring.
-        enough (Z.to_nat (word.unsigned num_bytes) <= length buf)%nat by blia.
-        PreOmega.zify. rewrite ?Znat.Z2Nat.id by eapply word.unsigned_range; blia. }
-      right. right. split; eauto using TracePredicate__any_app_more. } }
-
-
-  all: repeat letexists; split; repeat straightline;
-    eexists _, _; split; [ exact eq_refl | ].
-  all: eexists; split;
-    [repeat match goal with |- context [?x] => match type of x with list _ => subst x end end;
-    rewrite ?List.app_assoc; eauto|].
-  all: eexists; split;
-    [repeat eapply List.Forall2_app; eauto|].
-  all:
-    right; subst err;
-    split; [intro HX; inversion HX|].
-  all : repeat ((eexists; split; [solve[eauto]|]) || (split; [solve[eauto]|])).
-
-  (* two cases of SPI timeout *)
-  { left; split; [exact eq_refl|] || right.
-    left; split; [exact eq_refl|] || right.
-          split; [exact eq_refl|].
-      intuition eauto using TracePredicate__any_app_more. }
-  { left; split; [exact eq_refl|] || right.
-    left; split; [exact eq_refl|] || right.
-          split; [exact eq_refl|].
-      intuition eauto using TracePredicate__any_app_more. }
-  { left; split; [exact eq_refl|] || right.
-    left; split; [exact eq_refl|].
-    eexists _, _; split.
-    1:eapply TracePredicate.concat_app; try intuition eassumption.
-    subst v0.
-    rewrite word.unsigned_ltu in H6.
-    destruct (word.unsigned num_bytes <? word.unsigned (word.of_Z 1521)) eqn:?; try inversion H6.
-    eapply Z.ltb_nlt in Heqb; revert Heqb.
-    repeat match goal with |- context [?x] => match type of x with _ => subst x end end.
-    cbv [lan9250_decode_length]. split. 2: cbn in *; blia.
-    subst v. rewrite word.unsigned_and_nowrap in H2. eapply H2. }
-  { left.
-    split; [exact eq_refl|].
-    eexists; split; intuition eauto. }
-
-  Unshelve.
-  exact _.
-Defined.
-
-Import SPI.
-
-Definition function_impls :=
-  [lightbulb_init; lan9250_init; lan9250_wait_for_boot; lan9250_mac_write;
-  lightbulb_loop; lightbulb_handle; recvEthernet;  lan9250_writeword; lan9250_readword;
-  spi_xchg; spi_write; spi_read].
-
-Lemma link_lightbulb_loop : spec_of_lightbulb_loop function_impls.
-Proof.
-  eapply lightbulb_loop_ok;
-  (eapply recvEthernet_ok || eapply lightbulb_handle_ok);
-      eapply lan9250_readword_ok; eapply spi_xchg_ok;
-      (eapply spi_write_ok || eapply spi_read_ok).
-Qed.
-Lemma link_lightbulb_init : spec_of_lightbulb_init function_impls.
-Proof.
-Admitted.
-
-
-(* Print Assumptions link_lightbulb. *)
-(* parameters_ok FE310CSemantics.parameters, SortedList.TODO, TailRecursion.putmany_gather, SortedListString.string_strict_order *)
-
-From bedrock2 Require Import ToCString.
-Goal True.
-  let c_code := eval cbv in ((* of_string *) (@c_module BasicCSyntax.to_c_parameters function_impls)) in
-  pose c_code.
-Abort.
-
-(*
-From bedrock2 Require Import ToCString Byte Bytedump.
-Local Open Scope bytedump_scope.
-Set Printing Width 999999.
-Goal True.
-  let c_code := eval cbv in (of_string (@c_module BasicCSyntax.to_c_parameters [lan9250_init; lan9250_wait_for_boot; lightbulb_loop; lightbulb_handle; recvEthernet; lan9250_mac_write; lan9250_writeword; lan9250_readword; SPI.spi_xchg; SPI.spi_read; SPI.spi_write])) in
-  idtac c_code.
-Abort.
-*)
+        { repeat match goal with |- context [?x] => is_var x; subst x end.
+          rewrite word.unsigned_add. unfold word.wrap. rewrite Z.mod_small.
+          { replace (word.unsigned (word.of_Z 4)) with 4 by (rewrite word.unsigned_of_Z; exact eq_refl). blia. }
+          replace (word.unsigned (word.of_Z 4)) with 4 by (rewrite word.unsigned_of_Z; exact eq_refl).
+          Z.div_mod_to_equations. blia. }
+        { subst v'. subst i.
+          rewrite word.unsigned_add.
+          replace (word.unsigned (word.of_Z 4)) with 4 by (rewrite word.unsigned_of_Z; exact eq_refl).
+          unfold word.wrap. rewrite (Z.mod_small _ (2 ^ width));
+            change (2^width) with (2^32) in *; Z.div_mod_to_equations; blia. }
+  
+        { letexists; repeat split.
+          { repeat match goal with x := _ |- _ => is_var x; subst x end; subst.
+            cbv [scalar32 truncated_scalar littleendian ptsto_bytes.ptsto_bytes] in *.
+            progress replace (word.add x9 (word.add x11 (word.of_Z 4))) with
+                    (word.add (word.add x9 x11) (word.of_Z 4)) in * by ring.
+            SeparationLogic.seprewrite_in (@bytearray_index_merge) H25.
+            { rewrite word.unsigned_of_Z; exact eq_refl. } { ecancel_assumption. } }
+          { subst RECV. rewrite List.app_length.
+            rewrite H26. subst x22. rewrite List.length_skipn.
+            unshelve erewrite (_ : length (HList.tuple.to_list _) = 4%nat); [exact eq_refl|].
+            enough ((4 <= length x7)%nat) by blia.
+            Z.div_mod_to_equations; blia. }
+          repeat match goal with x := _ |- _ => is_var x; subst x end; subst.
+          eexists; split.
+          { rewrite List.app_assoc; eauto. }
+          eexists; split.
+          { eapply List.Forall2_app; eauto.  }
+          destruct H29; [left|right]; repeat (straightline || split || eauto using TracePredicate__any_app_more).
+          eapply TracePredicate.concat_app; eauto.
+          unshelve erewrite (_ : LittleEndian.combine _ _ = word.unsigned x10); rewrite !word.of_Z_unsigned; try solve [intuition idtac].
+          1: replace (word.unsigned x10) with (word.unsigned x10 mod 2^(Z.of_nat (bytes_per (width:=32) access_size.four)*8)).
+          1:rewrite <-LittleEndian.combine_split; f_equal.
+          eapply Properties.word.wrap_unsigned. } }
+  
+      { split; eauto. eexists; split; eauto. split; eauto. exists nil; split; eauto.
+        eexists; split; [constructor|].
+        left. split; eauto.
+        enough (Hlen : length x7 = 0%nat) by (destruct x7; try solve[inversion Hlen]; exact eq_refl).
+        PreOmega.zify.
+        rewrite H13.
+        subst br.
+        rewrite word.unsigned_ltu in H11.
+        destruct (word.unsigned x11 <? word.unsigned num_bytes) eqn:HJ.
+        { rewrite word.unsigned_of_Z in H11. inversion H11. }
+        eapply Z.ltb_nlt in HJ.
+        revert dependent x7; revert dependent num_bytes; revert dependent x11; clear; intros.
+        unshelve erewrite (_:x11 = num_bytes) in *.
+        { eapply Properties.word.unsigned_inj. Z.div_mod_to_equations; Lia.lia. }
+        rewrite word.unsigned_sub, Z.sub_diag; exact eq_refl. }
+      repeat straightline.
+      repeat letexists. split. { repeat straightline. }
+      eexists _, _. split. { exact eq_refl. }
+  
+      repeat straightline.
+      subst i.
+      match goal with H: _ |- _ =>
+        progress repeat (unshelve erewrite (_ : forall x, word.add x (word.of_Z 0) = x) in H; [intros; ring|]);
+        progress repeat (unshelve erewrite (_ : forall x, word.sub x (word.of_Z 0) = x) in H; [intros; ring|])
+      end.
+      eexists; split.
+      1: { repeat match goal with |- context [?x] => match type of x with list _ => subst x end end.
+        repeat rewrite List.app_assoc. f_equal. }
+      eexists; split.
+      1:repeat eapply List.Forall2_app; eauto.
+      destruct H14; [left|right]; repeat straightline; repeat split; eauto.
+      { trans_ltu;
+        replace (word.unsigned (word.of_Z 1521)) with 1521 in *
+          by (rewrite word.unsigned_of_Z; exact eq_refl).
+          eexists _, _; repeat split.
+        { SeparationLogic.ecancel_assumption. }
+        { revert dependent x2. revert dependent x6. intros.
+          destruct H5; repeat straightline; try contradiction.
+          destruct H9; repeat straightline; try contradiction.
+          eexists _, _; split.
+          { rewrite <-!List.app_assoc. eauto using concat_app. }
+          split; [zify_unsigned; eauto|].
+        { cbv beta delta [lan9250_decode_length].
+          rewrite H11. rewrite List.firstn_length, Znat.Nat2Z.inj_min.
+          replace (word.sub num_bytes (word.of_Z 0)) with num_bytes by ring.
+          rewrite ?Znat.Z2Nat.id by eapply word.unsigned_range.
+          transitivity (word.unsigned num_bytes); [blia|exact eq_refl]. } }
+        { pose proof word.unsigned_range num_bytes.
+          rewrite length_skipn.
+          PreOmega.zify. rewrite ?Znat.Z2Nat.id in * by blia; blia. }
+        rewrite H11, length_firstn_inbounds, ?Znat.Z2Nat.id.
+        all : try (zify_unsigned;
+        try Lia.lia;
+        eapply Znat.Nat2Z.inj_le;
+        rewrite ?Znat.Z2Nat.id; Lia.lia).
+        }
+      { repeat match goal with H : _ |- _ => rewrite H; intro HX; solve[inversion HX] end. }
+      { trans_ltu;
+        replace (word.unsigned (word.of_Z 1521)) with 1521 in * by
+          (rewrite word.unsigned_of_Z; exact eq_refl).
+        eexists _; split; eauto; repeat split; try Lia.lia.
+        { SeparationLogic.seprewrite_in @bytearray_index_merge H10.
+          { rewrite H11.
+            1: replace (word.sub num_bytes (word.of_Z 0)) with num_bytes by ring.
+            rewrite List.length_firstn_inbounds, ?Znat.Z2Nat.id.
+            1:exact eq_refl.
+            1:eapply word.unsigned_range.
+            PreOmega.zify.
+            rewrite ?Znat.Z2Nat.id by eapply word.unsigned_range.
+            blia. }
+          eapply H15. }
+        { 1:rewrite List.app_length, List.length_skipn, H11, List.firstn_length.
+          replace (word.sub num_bytes (word.of_Z 0)) with num_bytes by ring.
+          enough (Z.to_nat (word.unsigned num_bytes) <= length buf)%nat by blia.
+          PreOmega.zify. rewrite ?Znat.Z2Nat.id by eapply word.unsigned_range; blia. }
+        right. right. split; eauto using TracePredicate__any_app_more. } }
+  
+    all: repeat letexists; split; repeat straightline;
+      eexists _, _; split; [ exact eq_refl | ].
+    all: eexists; split;
+      [repeat match goal with |- context [?x] => match type of x with list _ => subst x end end;
+      rewrite ?List.app_assoc; eauto|].
+    all: eexists; split;
+      [repeat eapply List.Forall2_app; eauto|].
+    all:
+      right; subst err;
+      split; [intro HX; rewrite word.unsigned_of_Z in HX; inversion HX|].
+    all : repeat ((eexists; split; [solve[eauto]|]) || (split; [solve[eauto]|])).
+    all : rewrite !word.unsigned_of_Z.
+  
+    (* two cases of SPI timeout *)
+    { left; split; [exact eq_refl|] || right.
+      left; split; [exact eq_refl|] || right.
+            split; [exact eq_refl|].
+        intuition eauto using TracePredicate__any_app_more. }
+    { left; split; [exact eq_refl|] || right.
+      left; split; [exact eq_refl|] || right.
+            split; [exact eq_refl|].
+        intuition eauto using TracePredicate__any_app_more. }
+    { left; split; [exact eq_refl|] || right.
+      left; split; [exact eq_refl|].
+      eexists _, _; split.
+      1:eapply TracePredicate.concat_app; try intuition eassumption.
+      subst v0.
+      rewrite word.unsigned_ltu in H6.
+      destruct (word.unsigned num_bytes <? word.unsigned (word.of_Z 1521)) eqn:?.
+      all : rewrite word.unsigned_of_Z in Heqb, H6; try inversion H6.
+      eapply Z.ltb_nlt in Heqb; revert Heqb.
+      repeat match goal with |- context [?x] => match type of x with _ => subst x end end.
+      cbv [lan9250_decode_length]. split. 2: cbn in *; blia.
+      subst v. rewrite word.unsigned_and_nowrap, word.unsigned_of_Z in H2. eapply H2. }
+    { left.
+      split; [exact eq_refl|].
+      eexists; split; intuition eauto. }
+  Defined.
+  
+  Import SPI.
+  
+  Definition function_impls :=
+    [lightbulb_init; lan9250_init; lan9250_wait_for_boot; lan9250_mac_write;
+    lightbulb_loop; lightbulb_handle; recvEthernet;  lan9250_writeword; lan9250_readword;
+    spi_xchg; spi_write; spi_read].
+  
+  Lemma link_lightbulb_loop : spec_of_lightbulb_loop function_impls.
+  Proof.
+    eapply lightbulb_loop_ok;
+    (eapply recvEthernet_ok || eapply lightbulb_handle_ok);
+        eapply lan9250_readword_ok; eapply spi_xchg_ok;
+        (eapply spi_write_ok || eapply spi_read_ok).
+  Qed.
+  Lemma link_lightbulb_init : spec_of_lightbulb_init function_impls.
+  Proof.
+  Admitted.
+  
+  
+  (* Print Assumptions link_lightbulb. *)
+  (* parameters_ok FE310CSemantics.parameters, SortedList.TODO, TailRecursion.putmany_gather, SortedListString.string_strict_order *)
+  
+  From bedrock2 Require Import ToCString.
+  Goal True.
+    let c_code := eval cbv in ((* of_string *) (@c_module BasicCSyntax.to_c_parameters function_impls)) in
+    pose c_code.
+  Abort.
+  
+  (*
+  From bedrock2 Require Import ToCString Byte Bytedump.
+  Local Open Scope bytedump_scope.
+  Set Printing Width 999999.
+  Goal True.
+    let c_code := eval cbv in (of_string (@c_module BasicCSyntax.to_c_parameters [lan9250_init; lan9250_wait_for_boot; lightbulb_loop; lightbulb_handle; recvEthernet; lan9250_mac_write; lan9250_writeword; lan9250_readword; SPI.spi_xchg; SPI.spi_read; SPI.spi_write])) in
+    idtac c_code.
+  Abort.
+  *)
+End WithParameters.
